Added a basic implementation of BDDs as a HOL derived rule, in the new file Library/bdd.ml, together with some examples of usage in the other new file Examples/bdd_examples.ml The style of implementation follows Brace, Rudell and Bryant's paper "Efficient implementation of a BDD package" (DAC 1990). This implementation is distantly descended from the hol90 implementation in "Binary Decision Diagrams as a HOL Derived Rule", but greatly simplified since HOL Light handles pointer-eq subterms more efficiently and so we can avoid introducing any additional variables. Also added an extra utility function "atoms" for returning the set of propositional atomic formulas in a Boolean term.
Made a number of explicit type variable choices in theorems (and
occasionally fixed up or added quantifiers), just so things look
tidier with the new default print_types_of_subterms=1.

Added miscelleneous theorems, in particular quite a few connected
with the concept of "square-free":

        CARD_IMAGE_LE2
        CARD_IMAGE_LT2
        FORALL_PRIME_INDEX
        IMAGE_EQ
        ISOMORPHIC_PROD_INTEGER_MOD_RING
        RING_CARRIER_INTEGER_MOD_RING
        RING_HOMOMORPHISM_PROD_INTEGER_MOD_RING
        RING_ISOMORPHISM_PROD_INTEGER_MOD_RING
        RING_OF_INT_PROD_RING
        RING_OF_NUM_PROD_RING
        SQUAREFREE,SQUAREFREE_ALT
        SQUAREFREE_DIVEXP
        SQUAREFREE_DIVEXP_EQ
        SQUAREFREE_DIVIDES
        SQUAREFREE_GCD
        SQUAREFREE_GCD_SQUARE
        VNREGULAR_INTEGER_MOD_RING

Library/bdd.ml
@@ -1,0 +1,417 @@
+(* ========================================================================= *)
+(* Binary decision diagrams with complement edges, as a HOL derived rule.    *)
+(*                                                                           *)
+(* The style of implementation follows Brace, Rudell and Bryant's paper      *)
+(* "Efficient implementation of a BDD package" (DAC 1990). It's based on the *)
+(* hol90 implementation in "Binary Decision Diagrams as a HOL Derived Rule", *)
+(* but greatly simplified since HOL Light handles pointer-eq subterms more   *)
+(* efficiently and so we can avoid introducing any additional variables.     *)
+(* ========================================================================= *)
+
+let tfst (a,b,c) = a;;
+let tsnd (a,b,c) = b;;
+
+(* ------------------------------------------------------------------------- *)
+(* Handling of variable tables.                                              *)
+(* ------------------------------------------------------------------------- *)
+
+let var_of_num varray n = Array.get varray n;;
+
+let num_of_var (varray,vnext,vhash) v =
+  try Hashtbl.find vhash v
+  with Not_Found ->
+      let n = !vnext in
+      (vnext := n + 1; Array.set varray n v; Hashtbl.add vhash v n; n);;
+
+let mk_vtable n =
+  (Array.make (n+1) `T`,
+   ref 1,
+   (Hashtbl.create (n+1) :(term,int)Hashtbl.t));;
+
+(* ------------------------------------------------------------------------- *)
+(* Handling of unique table.                                                 *)
+(* ------------------------------------------------------------------------- *)
+
+let USIZE = 100000;;
+let UHASH = 1024;;
+
+let BDD_1 = USIZE + 1;;
+let BDD_0 = -BDD_1;;
+
+let btm_of_int =
+  let true_tm = `T` in
+  let rec btm_of_int uarray n =
+     if n < 0 then mk_neg(btm_of_int uarray (-n)) else
+     if n = BDD_1 then true_tm else
+     rand(rator(concl(snd(Array.get uarray n)))) in
+  btm_of_int;;
+
+let lookup_triple varray (uarray,unext,uhash) ((v,y,n) as tr) =
+  try Hashtbl.find uhash tr with Not_Found ->
+  let ytm = btm_of_int uarray y
+  and ntm = btm_of_int uarray n
+  and vtm = Array.get varray v
+  and m = !unext in
+  let ltm = mk_cond(vtm,ytm,ntm) in
+  let dth = REFL ltm in
+  (unext := m + 1;
+   Array.set uarray m (tr,dth);
+   Hashtbl.add uhash tr m;
+   m);;
+
+let bdd_expand uarray b =
+  if b < 0 then
+    let (v,l,r) = fst(Array.get uarray (-b)) in
+    (v,-l,-r)
+  else fst(Array.get uarray b);;
+
+let BDD_EXPAND =
+  let pth1 = TAUT
+    `~(if v then b1 else b2) <=> (if v then ~b1 else ~b2)`
+  and pth2 = TAUT
+    `~(if v then b1 else ~b2) <=> (if v then ~b1 else b2)`
+  and pth3 = TAUT
+    `~(if v then ~b1 else b2) <=> (if v then b1 else ~b2)`
+  and pth4 = TAUT
+    `~(if v then ~b1 else ~b2) <=> (if v then b1 else b2)`
+  and neg_tm = `~`
+  and v_tm = `v:bool`
+  and b1_tm = `b1:bool`
+  and b2_tm = `b2:bool` in
+  let rec BDD_EXPAND uarray b =
+    if b < 0 then
+      let def = snd(Array.get uarray (-b)) in
+      let (v,(y,n)) = dest_cond(rand(concl def)) in
+      let pth =
+        if is_neg y then
+          if is_neg n then INST [v,v_tm; rand y,b1_tm; rand n,b2_tm] pth4
+          else INST [v,v_tm; rand y,b1_tm; n,b2_tm] pth3
+        else
+          if is_neg n then INST [v,v_tm; y,b1_tm; rand n,b2_tm] pth2
+          else INST [v,v_tm; y,b1_tm; n,b2_tm] pth1 in
+      TRANS (AP_TERM neg_tm def) pth
+    else snd(Array.get uarray b) in
+  BDD_EXPAND;;
+
+let BDD_LOOKUP =
+  let pth1 = TAUT `b <=> (if v then b else b)`
+  and pth2 = TAUT
+    `(b <=> (if v then l else r))
+     ==> (~b <=> (if v then ~l else ~r))`
+  and pth3 = TAUT
+    `(b <=> (if v then l else ~r))
+     ==> (~b <=> (if v then ~l else r))`
+  and b_tm = `b:bool`
+  and v_tm = `v:bool`
+  and l_tm = `l:bool`
+  and r_tm = `r:bool` in
+  let rec BDD_LOOKUP varray utable (v,l,r) =
+    if l = r then
+      (INST [var_of_num varray v,v_tm;btm_of_int (tfst utable) l,b_tm] pth1,
+       l,0)
+    else if l < 0 then
+      let i = lookup_triple varray utable (v,-l,-r) in
+      let dth = snd(Array.get (tfst utable) i) in
+      let (ctm,(vtm,(ltm,rtm))) = (I F_F dest_cond) (dest_eq(concl dth)) in
+      if r < 0 then
+        (MP (INST [ctm,b_tm;vtm,v_tm;ltm,l_tm;rtm,r_tm] pth2) dth,-i,i)
+      else
+        (MP (INST [ctm,b_tm;vtm,v_tm;ltm,l_tm;rand rtm,r_tm] pth3) dth,-i,i)
+    else let i = lookup_triple varray utable (v,l,r) in
+         let dth = snd(Array.get (tfst utable) i) in
+         (dth,i,i) in
+  BDD_LOOKUP;;
+
+let mk_utable() =
+  (Array.make USIZE ((0,0,0),TRUTH),
+   ref 1,
+   (Hashtbl.create UHASH :(int*int*int,int)Hashtbl.t));;
+
+(* ------------------------------------------------------------------------- *)
+(* Handling of computed table.                                               *)
+(* ------------------------------------------------------------------------- *)
+
+let CSIZE = 200000;;
+let CHASH = 1024;;
+
+let bdd_and =
+  let pth1 = TAUT `~T /\ r1 <=> ~T`
+  and pth2 = TAUT `l1 /\ T <=> l1`
+  and pth3 = TAUT `l1 /\ l1 <=> l1`
+  and pth4 = TAUT `~r1 /\ r1 <=> ~T`
+  and pth5 = TAUT
+    `(b1 <=> (if v then l1 else r1))
+     ==> (b2 <=> (if v then l2 else r2))
+         ==> (b3 <=> (if v then l3 else r3))
+             ==> (l1 /\ l2 <=> l3) ==> (r1 /\ r2 <=> r3) ==> (b1 /\ b2 <=> b3)`
+  and pth6 = TAUT
+   `(b1 <=> (if v then l1 else r1))
+    ==> (b3 <=> (if v then l3 else r3))
+        ==> (l1 /\ b2 <=> l3) ==> (r1 /\ b2 <=> r3) ==> (b1 /\ b2 <=> b3)`
+  and pth7 = TAUT
+    `(b2 <=> (if v then l2 else r2))
+     ==> (b3 <=> (if v then l3 else r3))
+         ==> (b1 /\ l2 <=> l3) ==> (b1 /\ r2 <=> r3) ==> (b1 /\ b2 <=> b3)`
+  and pth8 = TAUT `l1 /\ r1 <=> r1 /\ l1`
+  and b1_tm = `b1:bool`
+  and b2_tm = `b2:bool`
+  and b3_tm = `b3:bool`
+  and l1_tm = `l1:bool`
+  and l2_tm = `l2:bool`
+  and l3_tm = `l3:bool`
+  and r1_tm = `r1:bool`
+  and r2_tm = `r2:bool`
+  and r3_tm = `r3:bool`
+  and v_tm = `v:bool`
+  and lookup_pair (carray,cnext,chash) (l,r) =
+     try let i = Hashtbl.find chash (l,r) in (fst(Array.get carray i),i)
+     with Not_Found -> failwith "lookup_pair" in
+  let rec bdd_and (varray,utable,((carray,cnext,chash) as ctable)) (l,r) =
+    try lookup_pair ctable (l,r) with Failure _ ->
+    let (ans,thm,uargs,cargs) =
+      if l = BDD_0 then
+       (BDD_0,INST [btm_of_int (tfst utable) r,r1_tm] pth1,[],[])
+      else if r = BDD_1 then
+       (l,INST [btm_of_int (tfst utable) l,l1_tm] pth2,[],[])
+      else if l = r then
+       (l,INST [btm_of_int (tfst utable) l,l1_tm] pth3,[],[])
+      else if l = -r then
+       (BDD_0,INST [btm_of_int (tfst utable) r,r1_tm] pth4,[],[])
+      else
+        let (lv,ly,ln) = bdd_expand (tfst utable) l
+        and (rv,ry,rn) = bdd_expand (tfst utable) r in
+        if lv = rv then
+          let (thy,cy,jy) = bdd_ands (varray,utable,ctable) (ly,ry) in
+          let (thn,cn,jn) = bdd_ands (varray,utable,ctable) (ln,rn) in
+          let thl = BDD_EXPAND (tfst utable) l in
+          let thr = BDD_EXPAND (tfst utable) r in
+          let (thc,c,jc) = BDD_LOOKUP varray utable (lv,cy,cn) in
+          let (b1,(v1,(l1,r1))) = (I F_F dest_cond) (dest_eq(concl thl)) in
+          let (b2,(v2,(l2,r2))) = (I F_F dest_cond) (dest_eq(concl thr)) in
+          let (b3,(v3,(l3,r3))) = (I F_F dest_cond) (dest_eq(concl thc)) in
+          let ith = INST [(b1,b1_tm);(b2,b2_tm);(b3,b3_tm);
+                          (l1,l1_tm);(l2,l2_tm);(l3,l3_tm);
+                          (r1,r1_tm);(r2,r2_tm);(r3,r3_tm);(v3,v_tm)] pth5 in
+          let lis = [thl; thr; thc; thy; thn] in
+          let xth = rev_itlist (C MP) lis ith in
+          (c,xth,[abs(l);abs(r);jc],[jy;jn])
+        else if lv > rv then
+          let (thy,cy,jy) = bdd_ands (varray,utable,ctable) (ly,r) in
+          let (thn,cn,jn) = bdd_ands (varray,utable,ctable) (ln,r) in
+          let thl = BDD_EXPAND (tfst utable) l in
+          let (thc,c,jc) = BDD_LOOKUP varray utable (lv,cy,cn) in
+          let (b1,(v1,(l1,r1))) = (I F_F dest_cond) (dest_eq(concl thl)) in
+          let (b3,(v3,(l3,r3))) = (I F_F dest_cond) (dest_eq(concl thc)) in
+          let b2 = rand(rand(rator(concl thy))) in
+          let ith = INST [(b1,b1_tm);(b2,b2_tm);(b3,b3_tm);
+                          (l1,l1_tm);(l3,l3_tm);
+                          (r1,r1_tm);(r3,r3_tm);(v3,v_tm)] pth6 in
+          let lis = [thl; thc; thy; thn] in
+          let xth = rev_itlist (C MP) lis ith in
+          (c,xth,[abs(l);jc],[jy;jn])
+        else
+          let (thy,cy,jy) = bdd_ands (varray,utable,ctable) (l,ry) in
+          let (thn,cn,jn) = bdd_ands (varray,utable,ctable) (l,rn) in
+          let thr = BDD_EXPAND (tfst utable) r in
+          let (thc,c,jc) = BDD_LOOKUP varray utable (rv,cy,cn) in
+          let (b2,(v2,(l2,r2))) = (I F_F dest_cond) (dest_eq(concl thr)) in
+          let (b3,(v3,(l3,r3))) = (I F_F dest_cond) (dest_eq(concl thc)) in
+          let b1 = rand(rator(rand(rator(concl thy)))) in
+          let ith = INST [(b1,b1_tm);(b2,b2_tm);(b3,b3_tm);
+                          (l2,l2_tm);(l3,l3_tm);
+                          (r2,r2_tm);(r3,r3_tm);(v3,v_tm)] pth7 in
+          let lis = [thr; thc; thy; thn] in
+          let xth = rev_itlist (C MP) lis ith in
+          (c,xth,[abs(r);jc],[jy;jn]) in
+    let m = !cnext in
+    (cnext := m + 1;
+     Array.set carray m ((ans,(thm,uargs,cargs)));
+     Hashtbl.add chash (l,r) m;
+     (ans,m))
+
+  and bdd_ands (varray,utable,ctable) (l,r) =
+    if (l:int) <= r then
+      let (ans,i) = bdd_and (varray,utable,ctable) (l,r) in
+      let th = tfst(snd(Array.get (tfst ctable) i)) in
+      (th,ans,i)
+    else
+      let (ans,i) = bdd_and (varray,utable,ctable) (r,l) in
+      let th = tfst(snd(Array.get (tfst ctable) i)) in
+      let ((ltm,rtm),ctm) = (dest_conj F_F I) (dest_eq(concl th)) in
+      let eth = INST [rtm,l1_tm; ltm,r1_tm] pth8 in
+      (TRANS eth th,ans,i) in
+  bdd_and;;
+
+let mk_ctable() =
+  (Array.make CSIZE (0,(TRUTH,([]:int list),([]:int list))),
+   ref 0,
+   (Hashtbl.create CHASH :(int*int,int)Hashtbl.t));;
+
+(* ------------------------------------------------------------------------- *)
+(* Basic BDD-constructing operations for the logical connectives.            *)
+(* ------------------------------------------------------------------------- *)
+
+let BDD_TRUE = (BDD_1,REFL `T`);;
+
+let BDD_FALSE = (BDD_0,TAUT `F <=> ~T`);;
+
+let BDD_VAR =
+  let pth = TAUT `(x <=> (if v then T else ~T)) ==> v = x`
+  and x_tm = `x:bool`
+  and v_tm = `v:bool` in
+  fun (vtable,utable,ctable) tm ->
+    let v = num_of_var vtable tm in
+    let u = lookup_triple (tfst vtable) utable (v,BDD_1,BDD_0) in
+    let ltm = btm_of_int (tfst utable) u in
+    let sth = INST [ltm,x_tm; tm,v_tm] pth in
+    let th = snd(Array.get (tfst utable) u) in
+    (u,MP sth th);;
+
+let BDD_NEG =
+  let neg_tm = `~`
+  and x_tm = `x:bool`
+  and pth = TAUT `~ ~ x <=> x` in
+  fun (vtable,utable,ctable) (i,fth) ->
+    if i < 0 then
+      let utm = btm_of_int (tfst utable) (-i) in
+      let th = INST [utm,x_tm] pth in
+      (-i,TRANS (AP_TERM neg_tm fth) th)
+    else
+      (-i,AP_TERM neg_tm fth);;
+
+let BDD_AND =
+  let and_tm = `/\`
+  and t1_tm = `t1:bool`
+  and t2_tm = `t2:bool` in
+  let pth = SPECL [t1_tm; t2_tm] CONJ_SYM in
+  fun (vtable,utable,ctable) ((i1,th1),(i2,th2)) ->
+    if i2 < i1 then
+      let (i3,j) = bdd_and (tfst vtable,utable,ctable) (i2,i1) in
+      let sth = INST [btm_of_int (tfst utable) i1,t1_tm;
+                      btm_of_int (tfst utable) i2,t2_tm] pth
+      and th = tfst(snd(Array.get (tfst ctable) j)) in
+      (i3,TRANS (MK_COMB(AP_TERM and_tm th1,th2))
+                (TRANS sth th))
+    else
+      let (i3,j) = bdd_and (tfst vtable,utable,ctable) (i1,i2) in
+      let th = tfst(snd(Array.get (tfst ctable) j)) in
+      (i3,TRANS (MK_COMB(AP_TERM and_tm th1,th2)) th);;
+
+let BDD_OR =
+  let pth = TAUT `~(~a /\ ~b) <=> a \/ b` in
+  let rew = REWR_CONV pth in
+  let rewl = LAND_CONV rew in
+  let rule = CONV_RULE rewl in
+  fun tt (b1,b2) ->
+    let (i,fth) = BDD_NEG tt (BDD_AND tt (BDD_NEG tt b1,BDD_NEG tt b2)) in
+    (i,rule fth);;
+
+let BDD_IMP =
+  let pth = TAUT `~(a /\ ~b) <=> a ==> b` in
+  let rew = REWR_CONV pth in
+  let rewl = LAND_CONV rew in
+  let rule = CONV_RULE rewl in
+  fun tt (b1,b2) ->
+    let (i,fth) = BDD_NEG tt (BDD_AND tt (b1,BDD_NEG tt b2)) in
+    (i,rule fth);;
+
+let BDD_IFF =
+  let pth = TAUT `~(a /\ ~b) /\ ~(~a /\ b) <=> (a <=> b)` in
+  let rew = REWR_CONV pth in
+  let rewl = LAND_CONV rew in
+  let rule = CONV_RULE rewl in
+  fun tt (b1,b2) ->
+    let (i,fth) = BDD_AND tt (BDD_NEG tt (BDD_AND tt (b1,BDD_NEG tt b2)),
+                            BDD_NEG tt (BDD_AND tt (BDD_NEG tt b1,b2))) in
+    (i,rule fth);;
+
+let rec BDD_OF_TERM defs tt tm =
+  match tm with
+    Const("T",_) -> BDD_TRUE
+  | Const("F",_) -> BDD_FALSE
+  | Comb(Comb(Const("/\\",_),l),r) ->
+        BDD_AND tt (BDD_OF_TERM defs tt l,BDD_OF_TERM defs tt r)
+  | Comb(Comb(Const("\\/",_),l),r) ->
+        BDD_OR tt (BDD_OF_TERM defs tt l,BDD_OF_TERM defs tt r)
+  | Comb(Comb(Const("==>",_),l),r) ->
+        BDD_IMP tt (BDD_OF_TERM defs tt l,BDD_OF_TERM defs tt r)
+  | Comb(Comb(Const("=",Tyapp("fun",[Tyapp("bool",[]);_])),l),r) ->
+        BDD_IFF tt (BDD_OF_TERM defs tt l,BDD_OF_TERM defs tt r)
+  | Comb(Const("~",_),l) ->
+        BDD_NEG tt (BDD_OF_TERM defs tt (rand tm))
+  | _ -> (try apply defs tm with Failure _ -> BDD_VAR tt tm);;
+
+(* ------------------------------------------------------------------------- *)
+(* Provide some information on output when verbose = 1                       *)
+(* ------------------------------------------------------------------------- *)
+
+let bdd_stats nd (vt,ct,ut) =
+  let d = if nd = 0 then "" else string_of_int nd^" definitions, " in
+  remark
+   ("BDD with "^d^
+    string_of_int(!(tsnd vt)) ^ " variables, " ^
+    string_of_int(!(tsnd ut)) ^ " nodes and " ^
+    string_of_int(!(tsnd ct)) ^ " cached results");;
+
+(* ------------------------------------------------------------------------- *)
+(* Basic tautology prover                                                    *)
+(* ------------------------------------------------------------------------- *)
+
+let BDD_TAUT tm =
+  let vt = mk_vtable(length(atoms tm))
+  and ut = mk_utable() and ct = mk_ctable() in
+  let b = BDD_OF_TERM undefined (vt,ut,ct) tm in
+  let _ = bdd_stats 0 (vt,ct,ut) in
+  EQT_ELIM (snd b);;
+
+(* ------------------------------------------------------------------------- *)
+(* A version that treats an input p ==> q specially, considering p           *)
+(* as a list of "definitions" (required to be left-to-right acyclic)         *)
+(* ------------------------------------------------------------------------- *)
+
+let BDD_DEFTAUT =
+  let bdd_def th =
+    let rule = TRANS th in
+    fun (i,fth) -> (i,rule fth) in
+  let rec bdd_of_defs defs tt ths =
+    match ths with
+      [] -> defs
+    | th::oths ->
+          let lv,rt = dest_eq(concl th) in
+          let br = BDD_OF_TERM defs tt rt in
+          let bl = bdd_def th br in
+          bdd_of_defs ((lv |-> bl) defs) tt oths in
+  let is_atomic tm =
+    not(is_neg tm || is_conj tm || is_disj tm || is_imp tm || is_iff tm) in
+  let is_literal tm =
+    (is_neg tm && is_atomic(rand tm)) || is_atomic tm in
+  let valid_definition tm =
+    (is_iff tm && is_literal(lhand tm)) || is_literal tm in
+  let ADJUST_DEF th =
+    let tm = concl th in
+    if is_neg tm then EQF_INTRO th
+    else if is_iff tm then th
+    else EQT_INTRO th in
+  let rec acyclic oks tms =
+    match tms with
+      [] -> true
+    | tm::otms -> not (exists (free_in (lhs tm)) (rand tm::oks)) &&
+                  acyclic (tm::oks) otms in
+  let valid_definitions tm =
+    let tms = map (concl o ADJUST_DEF o ASSUME) (conjuncts tm) in
+    forall valid_definition tms && acyclic [] tms in
+  fun ivars tm ->
+    let vars = ivars @ subtract (atoms tm) ivars in
+    let vt = mk_vtable (length vars)
+    and ut = mk_utable() and ct = mk_ctable() in
+    let _ = do_list (ignore o BDD_VAR (vt,ut,ct)) ivars in
+    if is_imp tm && valid_definitions (lhand tm) then
+      let ths = map ADJUST_DEF (CONJUNCTS(ASSUME(lhand tm))) in
+      let defs = bdd_of_defs undefined (vt,ut,ct) ths in
+      let b = BDD_OF_TERM defs (vt,ut,ct) (rand tm) in
+      let _ = bdd_stats (length(dom defs)) (vt,ct,ut) in
+      DISCH (lhand tm) (EQT_ELIM(snd b))
+    else
+      let b = BDD_OF_TERM undefined (vt,ut,ct) tm in
+      let _ = bdd_stats 0 (vt,ct,ut) in
+      EQT_ELIM(snd b);;
